src/SoftBound/sbop_seop.v
@@ -1,0 +1,345 @@
+Add LoadPath "../ssa/ott".
+Add LoadPath "../ssa/monads".
+Add LoadPath "../ssa/compcert".
+Add LoadPath "../ssa".
+Add LoadPath "../../../theory/metatheory_8.3".
+Add LoadPath "../TV".
+Require Import ssa_def.
+Require Import ssa_lib.
+Require Import List.
+Require Export targetdata.
+Require Import monad.
+Require Import Arith.
+Require Import Metatheory.
+Require Import genericvalues.
+Require Import trace.
+Require Import symexe_def.
+Require Import ssa_props.
+Require Import assoclist.
+Require Import sb_def.
+
+Export LLVMsyntax.
+Export LLVMlib.
+
+Tactic Notation "sb_dbCmd_cases" tactic(first) tactic(c) :=
+  first;
+  [ c "dbBop" | c "dbBop_error" | c "dbFBop" | c "dbFBop_eror" |
+    c "dbExtractValue" | c "dbExtractValue_error" | 
+    c "dbInsertValue" | c "dbInsertValue_error" |
+    c "dbMalloc" | c "dbMalloc_error" | c "dbFree" | c "dbFree_error" |
+    c "dbAlloca" | c "dbAlloca_error" | 
+    c "dbLoad_nptr" | c "dbLoad_ptr" | c "dbLoad_abort" |
+    c "dbStore_nptr" | c "dbStore_ptr" | c "dbStore_abort" |  
+    c "dbGEP" | c "dbGEP_error" |
+    c "dbTrunc" | c "dbTrunc_error" |
+    c "dbExt" | c "dbExt_error" |
+    c "dbBitcast_nptr" | c "dbBitcast_ptr" | c "dbInttoptr" | c "dbOtherCast" |
+    c "dbCast_error" | 
+    c "dbIcmp" | c "dbIcmp_error" |
+    c "dbFcmp" | c "dbFcmp_error" | 
+    c "dbSelect_nptr" | c "dbSelect_ptr"| c "dbSelect_error" |
+    c "dbLib" | c "dbLib_error" ].
+
+Tactic Notation "sb_dbTerminator_cases" tactic(first) tactic(c) :=
+  first;
+  [ c "dbBranch" | c "dbBranch_uncond" ].
+
+Tactic Notation "sb_dbCmds_cases" tactic(first) tactic(c) :=
+  first;
+  [ c "dbCmds_nil" | c "dbCmds_cons" | c "dbCmds_cons_error" ].
+
+(****************************************************)
+(* sbop -> seop *)
+
+Ltac invert_prop_reg_metadata :=
+  match goal with
+  | [H : SoftBound.prop_reg_metadata _ _ _ _ _ = (_, _) |- _ ] =>
+      inversion H; subst; eauto
+  end.
+
+Lemma updateAddAL_if_commut : forall lc id0 TD cond gv2 gv1,
+  updateAddAL GenericValue lc id0 (if isGVZero TD cond then gv2 else gv1) =
+  if isGVZero TD cond then 
+    (updateAddAL GenericValue lc id0 gv2) else 
+    (updateAddAL GenericValue lc id0 gv1).
+Admitted.
+
+Lemma sbop_dbCmd__seop_dbCmd : forall TD lc rm als gl Mem MM c lc' rm' als' 
+    Mem' MM' tr r, 
+  SoftBound.dbCmd TD gl lc rm als Mem MM c lc' rm' als' Mem' MM' tr r ->
+  r = SoftBound.rok ->
+  SimpleSE.dbCmd TD gl lc als Mem c lc' als' Mem' tr.
+Proof.
+  intros TD lc rm als gl Mem0 MM0 c lc' rm' als' Mem' MM' tr r H.
+  (sb_dbCmd_cases (destruct H) Case); intro J; 
+    try solve [inversion J; invert_prop_reg_metadata | eauto].
+  Case "dbSelect_nptr".
+    unfold SoftBound.SELECT in H.
+    remember (getOperandValue TD Mem0 v0 lc gl) as R0.
+    remember (getOperandValue TD Mem0 v1 lc gl) as R1.
+    remember (getOperandValue TD Mem0 v2 lc gl) as R2.
+    destruct R0 as [cond |]; try solve [inversion H].
+    destruct R1 as [gv1 |]; try solve [inversion H].
+    destruct R2 as [gv2 |]; inversion H; subst.
+    rewrite updateAddAL_if_commut. eauto.
+
+  Case "dbSelect_ptr".
+    unfold SoftBound.SELECT in H.
+    remember (getOperandValue TD Mem0 v0 lc gl) as R0.
+    remember (getOperandValue TD Mem0 v1 lc gl) as R1.
+    remember (getOperandValue TD Mem0 v2 lc gl) as R2.
+    destruct R0 as [cond |]; try solve [inversion H].
+    destruct R1 as [gv1 |]; try solve [inversion H].
+    destruct R2 as [gv2 |]; inversion H; subst.
+    inversion H3; subst.
+    assert (lc'=if isGVZero TD cond0 then updateAddAL _ lc id0 gv2
+                                     else updateAddAL _ lc id0 gv1) as EQ.
+      remember (isGVZero TD cond0) as R3.
+      destruct R3; inversion H4; subst; auto.
+    rewrite EQ. eauto.
+Qed.
+  
+Ltac invert_result :=
+  match goal with
+  | [H : SoftBound.is_error SoftBound.rok |- _ ] => inversion H
+  | [H : SoftBound.rerror = SoftBound.rok |- _ ] => inversion H
+  | [H : SoftBound.rabort = SoftBound.rok |- _ ] => inversion H 
+  | [H : SoftBound.rok = SoftBound.rerror |- _ ] => inversion H 
+  | [H : SoftBound.rok = SoftBound.rabort |- _ ] => inversion H 
+ end.
+
+Lemma sbop_dbCmds__seop_dbCmds : forall TD lc rm als gl Mem MM cs lc' rm' 
+    als' Mem' MM' tr r,
+  SoftBound.dbCmds TD gl lc rm als Mem MM cs lc' rm' als' Mem' MM' tr r ->
+  r = SoftBound.rok ->
+  SimpleSE.dbCmds TD gl lc als Mem cs lc' als' Mem' tr.
+Proof.
+  intros TD lc rm als gl Mem0 MM0 cs lc' rm' als' Mem' MM' tr r H.
+  (sb_dbCmds_cases (induction H) Case); intros J; subst;
+    try solve [invert_result | eauto using sbop_dbCmd__seop_dbCmd].
+Qed.
+
+Lemma sbop_callUpdateLocals__seop_callUpdateLocals : forall TD Mem'' noret0 rid 
+  oResult rm rm' lc lc' gl lc'' rm'',
+  SoftBound.callUpdateLocals TD Mem'' noret0 rid oResult rm rm' lc lc' gl = 
+    ret (lc'', rm'') ->
+  callUpdateLocals TD Mem'' noret0 rid oResult lc lc' gl = ret lc''.
+Proof.
+  intros. 
+  unfold SoftBound.callUpdateLocals in H.
+  unfold callUpdateLocals.
+  destruct noret0; try solve [inversion H; subst; auto].
+  destruct oResult; try solve [inversion H; subst; auto].
+  destruct (getOperandValue TD Mem'' v lc' gl); 
+    try solve [inversion H; subst; auto].
+  destruct (SoftBound.get_reg_metadata TD Mem'' gl rm' v);
+    try solve [inversion H; subst; auto].
+Qed.
+
+Definition sbop_dbCall__seop_dbCall_prop S TD Ps fs gl lc rm Mem0 MM0 call0 lc'
+rm' Mem' MM' tr r 
+(db:SoftBound.dbCall S TD Ps fs gl lc rm Mem0 MM0 call0 lc' rm' Mem' MM' tr r) :=
+  r = SoftBound.rok ->
+  SimpleSE.dbCall S TD Ps fs gl lc Mem0 call0 lc' Mem' tr.
+
+Definition sbop_dbSubblock__seop_dbSubblock_prop S TD Ps fs gl lc rm als Mem MM 
+cs lc' rm' als' Mem' MM' tr r
+(db:SoftBound.dbSubblock S TD Ps fs gl lc rm als Mem MM cs lc' rm' als' Mem' MM' 
+    tr r) :=
+  r = SoftBound.rok ->
+  SimpleSE.dbSubblock S TD Ps fs gl lc als Mem cs lc' als' Mem' tr.
+
+Definition sbop_dbSubblocks__seop_dbSubblocks_prop S TD Ps fs gl lc rm als Mem MM
+cs lc' rm' als' Mem' MM' tr r 
+(db:SoftBound.dbSubblocks S TD Ps fs gl lc rm als Mem MM cs lc' rm' als' Mem' MM'
+  tr r) :=
+  r = SoftBound.rok ->
+  SimpleSE.dbSubblocks S TD Ps fs gl lc als Mem cs lc' als' Mem' tr.
+
+Definition sbop_dbBlock__seop_dbBlock_prop S TD Ps fs gl F state state' tr r
+  (db:SoftBound.dbBlock S TD Ps fs gl F state state' tr r) :=
+  forall l ps cs tmn lc rm als Mem MM l' ps' cs' tmn' lc' rm' als' Mem' MM',
+  r = SoftBound.rok ->
+  state = SoftBound.mkState (SoftBound.mkEC (block_intro l ps cs tmn) lc rm als) 
+    Mem MM ->
+  state' = SoftBound.mkState (SoftBound.mkEC (block_intro l' ps' cs' tmn') lc' 
+    rm' als') Mem' MM' ->
+  SimpleSE.dbBlock S TD Ps fs gl F 
+    (SimpleSE.mkState (SimpleSE.mkEC (block_intro l ps cs tmn) lc als) Mem)
+    (SimpleSE.mkState (SimpleSE.mkEC (block_intro l' ps' cs' tmn') lc' 
+    als') Mem') tr.
+
+Definition sbop_dbBlocks__seop_dbBlocks_prop S TD Ps fs gl F state state' tr r
+  (db:SoftBound.dbBlocks S TD Ps fs gl F state state' tr r) :=
+  forall l ps cs tmn lc rm als Mem MM l' ps' cs' tmn' lc' rm' als' Mem' MM',
+  r = SoftBound.rok ->
+  state = SoftBound.mkState (SoftBound.mkEC (block_intro l ps cs tmn) lc rm als)
+    Mem MM ->
+  state' = SoftBound.mkState (SoftBound.mkEC (block_intro l' ps' cs' tmn') lc' 
+    rm' als') Mem' MM' ->
+  SimpleSE.dbBlocks S TD Ps fs gl F 
+    (SimpleSE.mkState (SimpleSE.mkEC (block_intro l ps cs tmn) lc als) Mem) 
+    (SimpleSE.mkState (SimpleSE.mkEC (block_intro l' ps' cs' tmn') lc' 
+    als') Mem') tr.
+
+Definition sbop_dbFdef__seop_dbFdef_prop fid rt lp S TD Ps lc rm gl fs Mem MM lc'
+  rm' als' Mem' MM' B' Rid oResult tr r
+  (db:SoftBound.dbFdef fid rt lp S TD Ps lc rm gl fs Mem MM lc' rm' als' Mem' MM'
+    B' Rid oResult tr r) :=
+  r = SoftBound.rok ->
+  SimpleSE.dbFdef fid rt lp S TD Ps lc gl fs Mem lc' als' Mem' B' Rid oResult
+    tr.
+
+Tactic Notation "sb_db_mutind_cases" tactic(first) tactic(c) :=
+  first;
+  [ c "dbCall_internal" | c "dbCall_external" |
+    c "dbCall_internal_error1" | c "dbCall_internal_error2" |
+    c "dbCall_external_error1" | c "dbCall_external_error2" |
+    c "dbSubblock_ok" | c "dbSubblock_error" | 
+    c "dbSubblocks_nil" | c "dbSubblocks_cons" | c "dbSubblocks_cons_error" |
+    c "dbBlock_ok" | c "dbBlock_error1" | c "dbBlock_error2" | 
+    c "dbBlocks_nil" | c "dbBlocks_cons" | c "dbBlocks_cons_error" | 
+    c "dbFdef_func" | c "dbFdef_func_error1" | c "dbFdef_func_error2" |
+    c "dbFdef_func_error3" | c "dbFdef_func_error4" | c "dbFdef_func_error5" |
+    c "dbFdef_proc" | c "dbFdef_proc_error1" | c "dbFdef_proc_error2" |
+    c "dbFdef_proc_error3" | c "dbFdef_proc_error4" | c "dbFdef_proc_error5"
+  ].
+
+Lemma sbop__seop :
+  (forall S TD Ps fs gl lc rm Mem0 MM0 call0 lc' rm' Mem' MM' tr r db, 
+     sbop_dbCall__seop_dbCall_prop S TD Ps fs gl lc rm Mem0 MM0 call0 lc' rm' 
+       Mem' MM' tr r db) 
+    /\
+  (forall S TD Ps fs gl lc rm als Mem MM sb lc' rm' als' Mem' MM' tr r db,
+     sbop_dbSubblock__seop_dbSubblock_prop S TD Ps fs gl lc rm als Mem MM sb lc' 
+       rm' als' Mem' MM' tr r db) /\
+  (forall S TD Ps fs gl lc rm als Mem MM sbs lc' rm' als' Mem' MM' tr r db,
+     sbop_dbSubblocks__seop_dbSubblocks_prop S TD Ps fs gl lc rm als Mem MM sbs 
+       lc' rm' als' Mem' MM' tr r db) /\
+  (forall S TD Ps fs gl F state1 state2 tr r db,
+     sbop_dbBlock__seop_dbBlock_prop S TD Ps fs gl F state1 state2 tr r db) /\
+  (forall S TD Ps fs gl F state1 state2 tr r db,
+     sbop_dbBlocks__seop_dbBlocks_prop S TD Ps fs gl F state1 state2 tr r db) /\
+  (forall fid rt lp S1 TD Ps1 lc rm gl fs Mem MM lc' rm' als' Mem' MM' B' Rid 
+       oResult tr r db,
+     sbop_dbFdef__seop_dbFdef_prop fid rt lp S1 TD Ps1 lc rm gl fs Mem MM lc' rm'
+       als' Mem' MM' B' Rid oResult tr r db).
+Proof.
+(sb_db_mutind_cases
+  apply SoftBound.sb_db_mutind with
+    (P  := sbop_dbCall__seop_dbCall_prop)
+    (P0 := sbop_dbSubblock__seop_dbSubblock_prop)
+    (P1 := sbop_dbSubblocks__seop_dbSubblocks_prop)
+    (P2 := sbop_dbBlock__seop_dbBlock_prop)
+    (P3 := sbop_dbBlocks__seop_dbBlocks_prop)
+    (P4 := sbop_dbFdef__seop_dbFdef_prop) Case);
+  unfold sbop_dbCall__seop_dbCall_prop, 
+         sbop_dbFdef__seop_dbFdef_prop, sbop_dbSubblock__seop_dbSubblock_prop,
+         sbop_dbSubblocks__seop_dbSubblocks_prop, 
+         sbop_dbBlock__seop_dbBlock_prop,
+         sbop_dbBlocks__seop_dbBlocks_prop; intros; subst; 
+    try solve [ invert_result | 
+                eauto using sbop_dbCmds__seop_dbCmds ].
+Case "dbCall_internal".
+  apply sbop_callUpdateLocals__seop_callUpdateLocals in e1; eauto.
+
+Case "dbBlock_ok".
+  inversion H1; subst. clear H1.
+  inversion H2; subst. clear H2.
+  apply sbop_dbCmds__seop_dbCmds in d0; eauto.
+
+Case "dbBlocks_nil".
+  inversion H1; subst. clear H1.
+  auto.
+
+Case "dbBlocks_cons".
+  inversion d; subst; try solve [ invert_result ].
+  destruct B'. eauto.
+Qed.
+
+Lemma sbop_dbCall__seop_dbCall : forall S TD Ps fs gl lc rm Mem0 MM0 call0 lc' 
+    rm' Mem' MM' tr,
+  SoftBound.dbCall S TD Ps fs gl lc rm Mem0 MM0 call0 lc' rm' Mem' MM' tr 
+    SoftBound.rok ->
+  SimpleSE.dbCall S TD Ps fs gl lc Mem0 call0 lc' Mem' tr.
+Proof.
+  intros.
+  destruct sbop__seop as [J _]. 
+  eapply J; eauto.
+Qed.
+
+Lemma sbop_dbSubblock__seop_dbSubblock : forall S TD Ps fs gl lc rm als Mem MM cs
+    lc' rm' als' Mem' MM' tr,
+  SoftBound.dbSubblock S TD Ps fs gl lc rm als Mem MM cs lc' rm' als' Mem' MM' tr
+    SoftBound.rok  ->
+  SimpleSE.dbSubblock S TD Ps fs gl lc als Mem cs lc' als' Mem' tr.
+Proof.
+  intros.
+  destruct sbop__seop as [_ [J _]]. 
+  eapply J; eauto.
+Qed.
+
+Lemma sbop_dbSubblocks__seop_dbSubblocks : forall S TD Ps fs gl lc rm als Mem MM 
+    cs lc' rm' als' Mem' MM' tr,
+  SoftBound.dbSubblocks S TD Ps fs gl lc rm als Mem MM cs lc' rm' als' Mem' MM' 
+    tr SoftBound.rok ->
+  SimpleSE.dbSubblocks S TD Ps fs gl lc als Mem cs lc' als' Mem' tr.
+Proof.
+  intros.
+  destruct sbop__seop as [_ [_ [J _]]]. 
+  eapply J; eauto.
+Qed.
+
+Lemma sbop_dbBlock__seop_dbBlock :  forall S TD Ps fs gl F tr l ps cs tmn lc rm 
+    als Mem MM l' ps' cs' tmn' lc' rm' als' Mem' MM',
+  SoftBound.dbBlock S TD Ps fs gl F 
+   (SoftBound.mkState (SoftBound.mkEC (block_intro l ps cs tmn) lc rm als) Mem 
+     MM) 
+   (SoftBound.mkState (SoftBound.mkEC (block_intro l' ps' cs' tmn') lc' rm' als')
+     Mem' MM') tr SoftBound.rok ->
+  SimpleSE.dbBlock S TD Ps fs gl F 
+    (SimpleSE.mkState (SimpleSE.mkEC (block_intro l ps cs tmn) lc als) Mem) 
+    (SimpleSE.mkState (SimpleSE.mkEC (block_intro l' ps' cs' tmn') lc' als') 
+    Mem') tr.
+Proof.
+  intros.
+  destruct sbop__seop as [_ [_ [_ [J _]]]]. 
+  eapply J; eauto.
+Qed.
+
+Lemma sbop_dbBlocks__seop_dbBlocks : forall S TD Ps fs gl F tr l ps cs tmn lc rm
+    als Mem MM l' ps' cs' tmn' lc' rm' als' Mem' MM',
+  SoftBound.dbBlocks S TD Ps fs gl F
+    (SoftBound.mkState (SoftBound.mkEC (block_intro l ps cs tmn) lc rm als) Mem 
+      MM) 
+    (SoftBound.mkState (SoftBound.mkEC (block_intro l' ps' cs' tmn') lc' rm' 
+      als') Mem' MM') tr SoftBound.rok ->  
+  SimpleSE.dbBlocks S TD Ps fs gl F
+    (SimpleSE.mkState (SimpleSE.mkEC (block_intro l ps cs tmn) lc als) Mem) 
+    (SimpleSE.mkState (SimpleSE.mkEC (block_intro l' ps' cs' tmn') lc' als') 
+      Mem') tr.
+Proof.
+  intros.
+  destruct sbop__seop as [_ [_ [_ [_ [J _]]]]]. 
+  eapply J; eauto.
+Qed.
+
+Lemma sbop_dbFdef__seop_dbFdef : forall fid rt lp S TD Ps lc rm gl fs Mem MM lc' 
+    rm' als' Mem' MM' B' Rid oResult tr,
+  SoftBound.dbFdef fid rt lp S TD Ps lc rm gl fs Mem MM lc' rm' als' Mem' MM' B'
+    Rid oResult tr SoftBound.rok ->
+  SimpleSE.dbFdef fid rt lp S TD Ps lc gl fs Mem lc' als' Mem' B' Rid oResult tr.
+Proof.
+  intros.
+  destruct sbop__seop as [_ [_ [_ [_ [_ J]]]]]. 
+  eapply J; eauto.
+Qed.
+
+(*****************************)
+(*
+*** Local Variables: ***
+*** coq-prog-name: "coqtop" ***
+*** coq-prog-args: ("-emacs-U" "-I" "~/SVN/sol/vol/src/ssa/monads" "-I" "~/SVN/sol/vol/src/ssa/ott" "-I" "~/SVN/sol/vol/src/ssa/compcert" "-I" "~/SVN/sol/theory/metatheory_8.3" "-I" "~/SVN/sol/vol/src/TV") ***
+*** End: ***
+ *)
+
